\documentclass{article}
\usepackage{amsmath}
\usepackage{amssymb}
\usepackage{amsthm}

\begin{document}

\section*{Problems}
\begin{enumerate}
\item $\displaystyle \lim_{x \to \infty} \frac{2x^3-4x+1}{x^3+5}$
\item $\displaystyle \lim_{x \to -\infty} -3x^4 + 8x^2 - 2x + 4$
\item $\displaystyle \lim_{x \to \infty} 2e^{-3x} - 4(2^x)$
\end{enumerate}


\section*{Solutions}
Let me solve these limits step by step.

1) $\displaystyle \lim_{x \to \infty} \frac{2x^3-4x+1}{x^3+5}$

For rational functions as x approaches infinity, we can divide both numerator and denominator by the highest power of x that appears (in this case, $x^3$).

$\displaystyle \lim_{x \to \infty} \frac{2x^3-4x+1}{x^3+5} = \lim_{x \to \infty} \frac{\frac{2x^3}{x^3}-\frac{4x}{x^3}+\frac{1}{x^3}}{\frac{x^3}{x^3}+\frac{5}{x^3}}$

$\displaystyle = \lim_{x \to \infty} \frac{2-\frac{4}{x^2}+\frac{1}{x^3}}{1+\frac{5}{x^3}}$

As $x \to \infty$, all terms with x in denominator approach 0.
Therefore, $\displaystyle \lim_{x \to \infty} \frac{2x^3-4x+1}{x^3+5} = 2$

2) $\displaystyle \lim_{x \to -\infty} -3x^4 + 8x^2 - 2x + 4$

For polynomial functions as x approaches infinity or negative infinity:
- The term with the highest degree determines the behavior
- If x approaches negative infinity and highest power is even, result is positive infinity

Here, highest power is 4 (even) and coefficient is -3 (negative)
Therefore, $\displaystyle \lim_{x \to -\infty} -3x^4 + 8x^2 - 2x + 4 = -\infty$

3) $\displaystyle \lim_{x \to \infty} 2e^{-3x} - 4(2^x)$

Let's analyze the two terms separately:
- $2e^{-3x}$ approaches 0 as $x \to \infty$ (negative exponent)
- $4(2^x)$ approaches $\infty$ as $x \to \infty$ (exponential growth)

Therefore, $\displaystyle \lim_{x \to \infty} 2e^{-3x} - 4(2^x) = 0 - \infty = -\infty$

The term $-4(2^x)$ dominates and since it's negative, the limit is negative infinity.
\end{document}